src/cbor/spec/raw/CBOR.Spec.API.Format.fst
@@ -1,0 +1,37 @@
+module CBOR.Spec.API.Format
+module RV = CBOR.Spec.Raw.Valid
+module RF = CBOR.Spec.Raw.Format
+module RS = CBOR.Spec.Raw.Sort
+module R = CBOR.Spec.Raw
+
+let cbor_parse x =
+  match RF.parse_cbor x with
+  | None -> None
+  | Some (y, n) ->
+    if RV.valid_raw_data_item y
+    then Some (R.mk_cbor y, n)
+    else None
+
+let cbor_parse_prefix x =
+  RF.parse_cbor_prefix x
+
+let cbor_det_serialize x =
+  RF.serialize_cbor (R.mk_det_raw_cbor x)
+
+let cbor_det_parse x =
+  match RF.parse_cbor x with
+  | None -> None
+  | Some (y, n) ->
+    if RV.raw_data_item_ints_optimal y && RS.raw_data_item_sorted RS.deterministically_encoded_cbor_map_key_order y
+    then begin
+      RV.raw_data_item_sorted_optimal_valid RS.deterministically_encoded_cbor_map_key_order y;
+      R.mk_det_raw_cbor_mk_cbor y;
+      Some (R.mk_cbor y, n)
+    end
+    else None
+
+let cbor_det_parse_prefix x =
+  RF.parse_cbor_prefix x
+
+let cbor_det_serialize_parse x =
+  RF.serialize_parse_cbor (R.mk_det_raw_cbor x)
